tests/test.c
@@ -6130,6 +6130,39 @@ int test_bignum_neg_p521(void)
   return 0;
 }
 
+int test_bignum_neg_sm2(void)
+{ uint64_t i, k;
+  printf("Testing bignum_neg_sm2 with %d cases\n",tests);
+  uint64_t c;
+  for (i = 0; i < tests; ++i)
+   { k = 4;
+     random_bignum(k,b2); reference_mod(k,b0,b2,p_sm2);
+     if ((rand() & 0x1F) == 0) reference_of_word(k,b0,0);
+
+     bignum_neg_sm2(b2,b0);
+     if (reference_iszero(k,b0)) reference_copy(k,b3,k,b0);
+     else reference_sub_samelen(k,b3,p_sm2,b0);
+
+     c = reference_compare(k,b3,k,b2);
+     if (c != 0)
+      { printf("### Disparity: [size %4"PRIu64"] "
+               "- ...0x%016"PRIx64" mod ....0x%016"PRIx64" = "
+               "...0x%016"PRIx64" not ...0x%016"PRIx64"\n",
+               k,b0[0],p_sm2[0],b2[0],b3[0]);
+        return 1;
+      }
+     else if (VERBOSE)
+      { if (k == 0) printf("OK: [size %4"PRIu64"]\n",k);
+        else printf("OK: [size %4"PRIu64"] "
+               "...0x%016"PRIx64" mod ....0x%016"PRIx64" = "
+               "...0x%016"PRIx64"\n",
+               k,b0[0],p_sm2[0],b2[0]);
+      }
+   }
+  printf("All OK\n");
+  return 0;
+}
+
 int test_bignum_negmodinv(void)
 { uint64_t t, i, k;
   printf("Testing bignum_negmodinv  with %d cases\n",tests);
@@ -9588,6 +9621,7 @@ int main(int argc, char *argv[])
   functionaltest(all,"bignum_neg_p256k1",test_bignum_neg_p256k1);
   functionaltest(all,"bignum_neg_p384",test_bignum_neg_p384);
   functionaltest(all,"bignum_neg_p521",test_bignum_neg_p521);
+  functionaltest(all,"bignum_neg_sm2",test_bignum_neg_sm2);
   functionaltest(all,"bignum_negmodinv",test_bignum_negmodinv);
   functionaltest(all,"bignum_nonzero",test_bignum_nonzero);
   functionaltest(all,"bignum_nonzero_4",test_bignum_nonzero_4);
