arm/proofs/bignum_neg_sm2.ml
@@ -4,81 +4,74 @@
  *)
 
 (* ========================================================================= *)
-(* Negation mod p_384, field characteristic for NIST P-384 curve.            *)
+(* Negation mod p_sm2, field characteristic for CC SM2 curve.                *)
 (* ========================================================================= *)
 
-(**** print_literal_from_elf "arm/p384/bignum_neg_p384.o";;
+(**** print_literal_from_elf "arm/sm2/bignum_neg_sm2.o";;
  ****)
 
-let bignum_neg_p384_mc = define_assert_from_elf "bignum_neg_p384_mc" "arm/p384/bignum_neg_p384.o"
+let bignum_neg_sm2_mc = define_assert_from_elf "bignum_neg_sm2_mc" "arm/sm2/bignum_neg_sm2.o"
 [
   0xa9401424;       (* arm_LDP X4 X5 X1 (Immediate_Offset (iword (&0))) *)
   0xa9411c26;       (* arm_LDP X6 X7 X1 (Immediate_Offset (iword (&16))) *)
-  0xa9422428;       (* arm_LDP X8 X9 X1 (Immediate_Offset (iword (&32))) *)
-  0xaa050082;       (* arm_ORR X2 X4 X5 *)
-  0xaa0700c3;       (* arm_ORR X3 X6 X7 *)
-  0xaa030042;       (* arm_ORR X2 X2 X3 *)
-  0xaa090103;       (* arm_ORR X3 X8 X9 *)
+  0xaa050083;       (* arm_ORR X3 X4 X5 *)
+  0xaa0700c2;       (* arm_ORR X2 X6 X7 *)
   0xaa030042;       (* arm_ORR X2 X2 X3 *)
   0xf100005f;       (* arm_CMP X2 (rvalue (word 0)) *)
   0xda9f03e2;       (* arm_CSETM X2 Condition_NE *)
-  0x92407c43;       (* arm_AND X3 X2 (rvalue (word 4294967295)) *)
-  0xeb040064;       (* arm_SUBS X4 X3 X4 *)
+  0xeb040044;       (* arm_SUBS X4 X2 X4 *)
   0x92607c43;       (* arm_AND X3 X2 (rvalue (word 18446744069414584320)) *)
   0xfa050065;       (* arm_SBCS X5 X3 X5 *)
-  0x927ff843;       (* arm_AND X3 X2 (rvalue (word 18446744073709551614)) *)
-  0xfa060066;       (* arm_SBCS X6 X3 X6 *)
-  0xfa070047;       (* arm_SBCS X7 X2 X7 *)
-  0xfa080048;       (* arm_SBCS X8 X2 X8 *)
-  0xda090049;       (* arm_SBC X9 X2 X9 *)
+  0xfa060046;       (* arm_SBCS X6 X2 X6 *)
+  0x925ff843;       (* arm_AND X3 X2 (rvalue (word 18446744069414584319)) *)
+  0xda070067;       (* arm_SBC X7 X3 X7 *)
   0xa9001404;       (* arm_STP X4 X5 X0 (Immediate_Offset (iword (&0))) *)
   0xa9011c06;       (* arm_STP X6 X7 X0 (Immediate_Offset (iword (&16))) *)
-  0xa9022408;       (* arm_STP X8 X9 X0 (Immediate_Offset (iword (&32))) *)
   0xd65f03c0        (* arm_RET X30 *)
 ];;
 
-let BIGNUM_NEG_P384_EXEC = ARM_MK_EXEC_RULE bignum_neg_p384_mc;;
+let BIGNUM_NEG_SM2_EXEC = ARM_MK_EXEC_RULE bignum_neg_sm2_mc;;
 
 (* ------------------------------------------------------------------------- *)
 (* Proof.                                                                    *)
 (* ------------------------------------------------------------------------- *)
 
-let p_384 = new_definition `p_384 = 39402006196394479212279040100143613805079739270465446667948293404245721771496870329047266088258938001861606973112319`;;
+let p_sm2 = new_definition `p_sm2 = 0xFFFFFFFEFFFFFFFFFFFFFFFFFFFFFFFFFFFFFFFF00000000FFFFFFFFFFFFFFFF`;;
 
-let BIGNUM_NEG_P384_CORRECT = time prove
+let BIGNUM_NEG_SM2_CORRECT = time prove
  (`!z x n pc.
-        nonoverlapping (word pc,0x5c) (z,8 * 6)
+        nonoverlapping (word pc,0x40) (z,8 * 4)
         ==> ensures arm
-             (\s. aligned_bytes_loaded s (word pc) bignum_neg_p384_mc /\
+             (\s. aligned_bytes_loaded s (word pc) bignum_neg_sm2_mc /\
                   read PC s = word pc /\
                   C_ARGUMENTS [z; x] s /\
-                  bignum_from_memory (x,6) s = n)
-             (\s. read PC s = word (pc + 0x58) /\
-                  (n <= p_384
-                   ==> bignum_from_memory (z,6) s = (p_384 - n) MOD p_384))
-          (MAYCHANGE [PC; X2; X3; X4; X5; X6; X7; X8; X9] ,,
+                  bignum_from_memory (x,4) s = n)
+             (\s. read PC s = word (pc + 0x3c) /\
+                  (n <= p_sm2
+                   ==> bignum_from_memory (z,4) s = (p_sm2 - n) MOD p_sm2))
+          (MAYCHANGE [PC; X2; X3; X4; X5; X6; X7] ,,
            MAYCHANGE SOME_FLAGS ,,
-           MAYCHANGE [memory :> bignum(z,6)])`,
+           MAYCHANGE [memory :> bignum(z,4)])`,
   MAP_EVERY X_GEN_TAC [`z:int64`; `x:int64`; `n:num`; `pc:num`] THEN
   REWRITE_TAC[C_ARGUMENTS; C_RETURN; SOME_FLAGS; NONOVERLAPPING_CLAUSES] THEN
   DISCH_THEN(REPEAT_TCL CONJUNCTS_THEN ASSUME_TAC) THEN
   REWRITE_TAC[BIGNUM_FROM_MEMORY_BYTES] THEN ENSURES_INIT_TAC "s0" THEN
-  BIGNUM_DIGITIZE_TAC "n_" `read (memory :> bytes (x,8 * 6)) s0` THEN
+  BIGNUM_DIGITIZE_TAC "n_" `read (memory :> bytes (x,8 * 4)) s0` THEN
 
-  ARM_ACCSTEPS_TAC BIGNUM_NEG_P384_EXEC [12;14;16;17;18;19] (1--22) THEN
+  ARM_ACCSTEPS_TAC BIGNUM_NEG_SM2_EXEC [8;10;11;13] (1--15) THEN
   ENSURES_FINAL_STATE_TAC THEN ASM_REWRITE_TAC[] THEN STRIP_TAC THEN
   CONV_TAC(LAND_CONV BIGNUM_EXPAND_CONV) THEN
-  ASM_REWRITE_TAC[] THEN DISCARD_STATE_TAC "s22" THEN
+  ASM_REWRITE_TAC[] THEN DISCARD_STATE_TAC "s15" THEN
   REWRITE_TAC[GSYM REAL_OF_NUM_CLAUSES] THEN
   MATCH_MP_TAC EQUAL_FROM_CONGRUENT_REAL THEN
-  MAP_EVERY EXISTS_TAC [`384`; `&0:real`] THEN
+  MAP_EVERY EXISTS_TAC [`256`; `&0:real`] THEN
   CONJ_TAC THENL [BOUNDER_TAC[]; ALL_TAC] THEN CONJ_TAC THENL
-   [UNDISCH_TAC `n <= p_384` THEN
-    REWRITE_TAC[REAL_OF_NUM_CLAUSES; p_384] THEN ARITH_TAC;
+   [UNDISCH_TAC `n <= p_sm2` THEN
+    REWRITE_TAC[REAL_OF_NUM_CLAUSES; p_sm2] THEN ARITH_TAC;
     ALL_TAC] THEN
   CONJ_TAC THENL [REAL_INTEGER_TAC; ALL_TAC] THEN
 
-  SUBGOAL_THEN `(p_384 - n) MOD p_384 = if n = 0 then 0 else p_384 - n`
+  SUBGOAL_THEN `(p_sm2 - n) MOD p_sm2 = if n = 0 then 0 else p_sm2 - n`
   SUBST1_TAC THENL
    [COND_CASES_TAC THEN ASM_REWRITE_TAC[SUB_0; MOD_REFL] THEN
     MATCH_MP_TAC MOD_LT THEN ASM_ARITH_TAC;
@@ -90,24 +83,24 @@ let BIGNUM_NEG_P384_CORRECT = time prove
   REWRITE_TAC[WORD_UNMASK_64; WORD_SUB_0; VAL_EQ_0] THEN
   REWRITE_TAC[WORD_AND_MASK; COND_SWAP; WORD_OR_EQ_0; VAL_EQ_0] THEN
   REWRITE_TAC[CONJ_ACI] THEN COND_CASES_TAC THEN
-  ASM_REWRITE_TAC[p_384; GSYM REAL_OF_NUM_CLAUSES; BITVAL_CLAUSES] THEN
+  ASM_REWRITE_TAC[p_sm2; GSYM REAL_OF_NUM_CLAUSES; BITVAL_CLAUSES] THEN
   CONV_TAC WORD_REDUCE_CONV THEN
   DISCH_THEN(fun th -> REWRITE_TAC[th]) THEN REAL_INTEGER_TAC);;
 
-let BIGNUM_NEG_P384_SUBROUTINE_CORRECT = time prove
+let BIGNUM_NEG_SM2_SUBROUTINE_CORRECT = time prove
  (`!z x n pc returnaddress.
-        nonoverlapping (word pc,0x5c) (z,8 * 6)
+        nonoverlapping (word pc,0x40) (z,8 * 4)
         ==> ensures arm
-             (\s. aligned_bytes_loaded s (word pc) bignum_neg_p384_mc /\
+             (\s. aligned_bytes_loaded s (word pc) bignum_neg_sm2_mc /\
                   read PC s = word pc /\
                   read X30 s = returnaddress /\
                   C_ARGUMENTS [z; x] s /\
-                  bignum_from_memory (x,6) s = n)
+                  bignum_from_memory (x,4) s = n)
              (\s. read PC s = returnaddress /\
-                  (n <= p_384
-                   ==> bignum_from_memory (z,6) s = (p_384 - n) MOD p_384))
-          (MAYCHANGE [PC; X2; X3; X4; X5; X6; X7; X8; X9] ,,
+                  (n <= p_sm2
+                   ==> bignum_from_memory (z,4) s = (p_sm2 - n) MOD p_sm2))
+          (MAYCHANGE [PC; X2; X3; X4; X5; X6; X7] ,,
            MAYCHANGE SOME_FLAGS ,,
-           MAYCHANGE [memory :> bignum(z,6)])`,
-  ARM_ADD_RETURN_NOSTACK_TAC BIGNUM_NEG_P384_EXEC
-      BIGNUM_NEG_P384_CORRECT);;
+           MAYCHANGE [memory :> bignum(z,4)])`,
+  ARM_ADD_RETURN_NOSTACK_TAC BIGNUM_NEG_SM2_EXEC
+      BIGNUM_NEG_SM2_CORRECT);;
